🧠 - somehow it works better after midnight

pset10_ProgramEquivalence/Pset10.v
@@ -24,7 +24,7 @@ Module Impl.
   (** * Object language (assembly-style) *)
 
   (* Let's define the very simple programming language we'll work with. *)
-  
+
   (** ** Syntax *)
 
   Inductive binop := Add | Mul | Sub.
@@ -112,7 +112,7 @@ Module Impl.
 
   (* OK, now we turn to the type of state that we maintain during symbolic
    * execution of programs. *)
-  
+
   Definition nodes_in := fmap node_kind node.
   Definition nodes_out := fmap node node_kind.
   Definition varmap := fmap var node.
@@ -121,10 +121,10 @@ Module Impl.
                       NodesIn : nodes_in;
                       (* Maps each node kind seen so far its unique
                        * identifier *)
-                      
+
                       NodesOut : nodes_out;
                       (* Dually, maps the identifiers back to their kinds *)
-                      
+
                       NextNode : node;
                       (* The next node identifier we'll use, when the time comes
                        * to generate a new one *)
@@ -307,7 +307,7 @@ Module Impl.
    * finite maps, which are actually axiomatized instead of defined
    * computationally, which prevents us from using the built-in interpreter to
    * do all of the execution work efficiently. *)
-   
+
   Example ex1a := [Instr "x" (Const 1);
                    Instr "y" (Const 2);
                    Instr "out" (Binop Add "x" "y")].
@@ -357,7 +357,7 @@ Module Impl.
 
   (* To make sure symbolic execution tracks enough variables, we need to define
    * which variables an instruction reads. *)
-  
+
   Definition rhsReads (r : rhs) : set var :=
     match r with
     | Const _ => {}
@@ -374,13 +374,999 @@ Module Impl.
    * variable reads depend on the initial values of variables. *)
 
 
+(* | We're glad to give full credit for any proof of the designated main theorem,
+  but it's a relatively involved proof, so we also give the great majority of a
+  solution below, with notes on how we will assign partial credit for the
+  unproved lemmas that we have left. *)
+
+  (* The following type will play a crucial role: it assigns semantic meanings
+   * to all graph nodes. *)
+  Definition nodeVals := fmap node Z.
+
+  (* Interpreting our node kinds w.r.t. node values and variable values is
+   * fairly straightforward. *)
+
+  Definition sum := fold_left Z.add.
+  Definition product := fold_left Z.mul.
+
+  Definition evalNodeKind (nvs : nodeVals) (v : valuation) (nk : node_kind) : Z :=
+    match nk with
+    | SConst n => n
+    | SVar x => v $! x
+    | SAdd n nds => sum (map (fun nd => nvs $! nd) nds) n
+    | SMul n nds => product (map (fun nd => nvs $! nd) nds) n
+    | SSub nd1 nd2 => nvs $! nd1 - nvs $! nd2
+    end.
+
+  (* It's useful to have a way to state bounds on which node identifiers may
+   * appear in a node kind. *)
+  Definition nodeKindInBounds (bound : Z) (nk : node_kind) :=
+    match nk with
+    | SConst _ | SVar _ => True
+    | SAdd _ args | SMul _ args => List.Forall (fun arg => arg < bound) args
+    | SSub x y => x < bound /\ y < bound
+    end.
+
+  (* Here is the main invariant we maintain as we execute, connecting: *)
+  Record compat
+         (st : sstate)      (* symbolic state *)
+         (v0 v : valuation) (* initial and current variable values *)
+         (nvs : nodeVals)   (* node values *) := {
+      OutToIn : forall nd nk, st.(NodesOut) $? nd = Some nk
+                              -> st.(NodesIn) $? nk = Some nd;
+      InToOut : forall nd nk, st.(NodesIn) $? nk = Some nd
+                              -> st.(NodesOut) $? nd = Some nk;
+      InBounds1 : forall nd nk, st.(NodesOut) $? nd = Some nk
+                                -> nd < st.(NextNode);
+      InBounds2 : forall nd nk, st.(NodesIn) $? nk = Some nd
+                                -> nodeKindInBounds st.(NextNode) nk;
+      OutVals : forall nd nk, st.(NodesOut) $? nd = Some nk
+                              -> nvs $? nd = Some (evalNodeKind nvs v0 nk);
+      OutValsInv : forall nd, nvs $? nd <> None
+                              -> st.(NodesOut) $? nd <> None;
+      VarToNode : forall x nd, st.(Vars) $? x = Some nd
+                             -> st.(NodesOut) $? nd <> None;
+      VarToNodevals : forall x nd, st.(Vars) $? x = Some nd
+                             -> nvs $? nd = Some (v $! x)
+    }.
+  (* Note that we have defined a predicate as a record, which basically means
+   * the predicate is a big "and" of the different named properties.  This
+   * syntax actually desugars into an inductive predicate definition with a
+   * single constructor, plus a projection function per record field.  Try
+   * [Check]ing the field names to see how that works. *)
+
+  Local Hint Resolve VarToNode : core.
+
+  Lemma varIsFine : forall (s : set var) (m : fmap var node) x,
+      s \subseteq dom m
+      -> m $? x = None
+      -> x \in s
+      -> False.
+  Proof.
+    simplify.
+    apply lookup_None_dom in H0.
+    sets.
+  Qed.
+
+  Local Hint Extern 1 False => (eapply varIsFine; [ eassumption | eassumption | sets ]) : core.
+
+  Lemma nvs_anything : forall (nvs : nodeVals) nd n,
+      nvs $? nd = Some n
+      -> nvs $? nd = Some (nvs $! nd).
+  Proof.
+    simplify.
+    rewrite H.
+    reflexivity.
+  Qed.
+
+  Local Hint Resolve nvs_anything : core.
+
+  (* OK, our first correctness theorem for a helper function: *)
+  (*[15%]*)Lemma symAddOf_correct : forall st v0 v nvs n z l,
+      compat st v0 v nvs
+      -> st.(NodesOut) $? n <> None
+      -> symAddOf st n = (z, l)
+      -> nvs $? n = Some (sum (map (fun nd => nvs $! nd) l) z).
+  Proof.
+    unfold symAddOf; simplify.
+    cases (st.(NodesOut) $? n); simplify.
+    - cases n0; simplify;
+      invert H1;
+      pose proof (OutVals st v0 v nvs H n _ Heq);
+      eauto.
+    - equality.
+  Qed.
+
+  (* Symmetrical one for multiplication: *)
+  (*[15%]*)Lemma symMulOf_correct : forall st v0 v nvs n z l,
+      compat st v0 v nvs
+      -> st.(NodesOut) $? n <> None
+      -> symMulOf st n = (z, l)
+      -> nvs $? n = Some (product (map (fun nd => nvs $! nd) l) z).
+  Proof.
+    unfold symMulOf; simplify.
+    cases (st.(NodesOut) $? n); simplify.
+    - cases n0; simplify;
+      invert H1;
+      pose proof (OutVals st v0 v nvs H n _ Heq);
+      eauto; simplify;
+      cases (nvs $! n); invert Heq0; eauto.
+    - equality.
+  Qed.
+
+  (* We will need to know that merging sums and products has the expected
+   * effects, and one way to go about it is proving properties generically for
+   * associative-commutative operators. *)
+  Section associative_commutative.
+    Variable f : Z -> Z -> Z.
+    Hypothesis commutative : forall x y, f x y = f y x.
+    Hypothesis associative : forall x y z, f (f x y) z = f x (f y z).
+
+    Variable g : Z -> Z.
+
+    Lemma fold_left_permutation : forall l l' a,
+        Permutation.Permutation l l' -> fold_left f l a = fold_left f l' a.
+    Proof.
+      simplify; revert a.
+      induction H; eauto; simplify.
+      - rewrite associative.
+        rewrite commutative.
+        rewrite associative.
+        rewrite (commutative a x).
+        rewrite commutative.
+        eauto.
+      - rewrite IHPermutation1, IHPermutation2; auto.
+    Qed.
+
+    Lemma fold_left_f_merge1 : forall l a b,
+        fold_left f l (f a b) = f (fold_left f l a) b.
+    Proof.
+      induction l; simpl; auto.
+      intros.
+      rewrite associative.
+      rewrite <-IHl.
+      rewrite associative.
+      rewrite (commutative b a).
+      eauto.
+    Qed.
+
+    Lemma fold_left_f_merge3 : forall l a b,
+        fold_left f l (f a b) = f a (fold_left f l b).
+    Proof.
+      intros.
+      rewrite commutative.
+      rewrite fold_left_f_merge1.
+      rewrite commutative.
+      eauto.
+    Qed.
+
+    Lemma merge_dumb: forall l,
+        ZSort.merge [] l = l.
+    Proof.
+      induct l.
+      - simplify; eauto.
+      - simplify; eauto.
+    Qed.
+
+    Lemma perm_swap_app : forall (A : Type) (x y : A) (l1 l2 : list A),
+        Permutation.Permutation (y :: x :: l1 ++ l2) (x :: l1 ++ y :: l2).
+    Proof.
+      simplify.
+      apply Permutation.perm_trans with (l' := x :: y :: l1 ++ l2).
+      - apply Permutation.perm_swap.
+      - rewrite app_comm_cons.
+        rewrite Permutation.perm_skip; eauto.
+        eapply Permutation.Permutation_cons_app; eauto.
+    Qed.
+
+
+    Lemma merge_permutation : forall l1 l2,
+        Permutation.Permutation (ZSort.merge l1 l2) (l1 ++ l2).
+    Proof.
+      induct l1; intros.
+      - replace ([] ++ l2) with l2 by (simplify; eauto).
+        rewrite merge_dumb.
+        eauto.
+      - induct l2.
+        + simplify. rewrite app_nil_r. apply Permutation.Permutation_refl.
+        + simpl.
+          destruct (Z.leb a a0).
+          ++ simplify. eapply Permutation.perm_skip. apply IHl1.
+          ++ eapply Permutation.perm_skip in IHl2.
+             simpl in IHl2.
+             eapply Permutation.perm_trans.
+             eapply IHl2.
+             eapply perm_swap_app.
+    Qed.
+
+    (*[35%]*)Lemma merge_combine : forall l1 n1 l2 n2,
+        fold_left f (map g (ZSort.merge l1 l2)) (f n1 n2)
+        = f (fold_left f (map g l1) n1) (fold_left f (map g l2) n2).
+    Proof.
+      intros.
+      rewrite fold_left_permutation with (l' := map g (l1 ++ l2)).
+      - rewrite map_app.
+        rewrite fold_left_app.
+        rewrite fold_left_f_merge1.
+        rewrite fold_left_f_merge3.
+        eauto.
+      - rewrite merge_permutation.
+        eauto.
+    Qed.
+
+    (* We proved this one via several more-general lemmas. *)
+  End associative_commutative.
+
+  Lemma VarVals3 : forall st v0 v nvs x n n1,
+      compat st v0 v nvs
+      -> Vars st $? x = Some n
+      -> NodesOut st $? n = Some n1
+      -> evalNodeKind nvs v0 n1 = v $! x.
+  Proof.
+    simplify.
+    eapply VarToNodevals in H0; eauto.
+    eapply OutVals in H1; eauto.
+    equality.
+  Qed.
+
+  Local Hint Resolve VarVals3 : core.
+
+
+  (* Another helper's correctness theorem *)
+  (*[35%]*)Lemma kindOfRhs_correct : forall st r nvs v0 v,
+      compat st v0 v nvs
+      -> rhsReads r \subseteq dom st.(Vars)
+      -> evalNodeKind nvs v0 (kindOfRhs st r) = evalRhs r v.
+  Proof.
+    simplify.
+    unfold kindOfRhs, evalRhs.
+
+    cases r; simplify.
+    - equality. (* "* = ++". "-- = ++" *)
+    - cases b; simplify.
+      + cases (Vars st $? x); simplify.
+        ++ cases (Vars st $? y); simplify.
+          -- cases (symAddOf st n).
+            cases (symAddOf st n0).
+            cases (isNil (ZSort.merge l l0)); simplify.
+            ---
+                pose proof (VarToNode st v0 v nvs H x n Heq).
+                pose proof (VarToNode st v0 v nvs H y n0 Heq0).
+                pose proof (symAddOf_correct st v0 v nvs n _ _ H H1 Heq1).
+                pose proof (symAddOf_correct st v0 v nvs n0 _ _ H H2 Heq2).
+                pose proof (VarToNodevals st v0 v nvs H x n Heq).
+                pose proof (VarToNodevals st v0 v nvs H y n0 Heq0).
+
+                rewrite H5 in H3.
+                rewrite H6 in H4.
+                invert H3.
+                invert H4.
+                rewrite H7, H8.
+
+                unfold sum.
+
+                unfold isNil in Heq3.
+                cases (ZSort.merge l l0).
+                assert (sum (map (fun nd : node => nvs $! nd) (ZSort.merge l l0)) (z+z0) = z+z0).
+                rewrite Heq4.
+                simplify.
+                equality.
+                invert H3.
+
+                eapply merge_combine.
+                simplify.
+                linear_arithmetic.
+
+                simplify.
+                linear_arithmetic.
+
+                exfalso. linear_arithmetic.
+            ---
+                pose proof (VarToNode st v0 v nvs H x n Heq).
+                pose proof (VarToNode st v0 v nvs H y n0 Heq0).
+                pose proof (symAddOf_correct st v0 v nvs n _ _ H H1 Heq1).
+                pose proof (symAddOf_correct st v0 v nvs n0 _ _ H H2 Heq2).
+                pose proof (VarToNodevals st v0 v nvs H x n Heq).
+                pose proof (VarToNodevals st v0 v nvs H y n0 Heq0).
+
+                rewrite H5 in H3.
+                rewrite H6 in H4.
+                invert H3.
+                invert H4.
+                rewrite H7, H8.
+                unfold sum.
+                eapply merge_combine; eauto; simplify; linear_arithmetic.
+          -- exfalso; eauto.
+        ++ exfalso; eauto.
+      + cases (Vars st $? x); simplify.
+        ++ cases (Vars st $? y); simplify.
+          -- cases (symMulOf st n).
+            cases (symMulOf st n0).
+            cases (isNil (ZSort.merge l l0)); simplify.
+            ---
+                pose proof (VarToNode st v0 v nvs H x n Heq).
+                pose proof (VarToNode st v0 v nvs H y n0 Heq0).
+                pose proof (symMulOf_correct st v0 v nvs n _ _ H H1 Heq1).
+                pose proof (symMulOf_correct st v0 v nvs n0 _ _ H H2 Heq2).
+                pose proof (VarToNodevals st v0 v nvs H x n Heq).
+                pose proof (VarToNodevals st v0 v nvs H y n0 Heq0).
+
+                rewrite H5 in H3.
+                rewrite H6 in H4.
+                invert H3.
+                invert H4.
+                rewrite H7, H8.
+
+                unfold product.
+                unfold isNil in Heq3.
+                cases (ZSort.merge l l0).
+
+                assert (product (map (fun nd : node => nvs $! nd) (ZSort.merge l l0)) (z*z0) = z*z0).
+                rewrite Heq4.
+                simplify.
+                equality.
+                invert H3.
+
+                eapply merge_combine.
+                simplify.
+                linear_arithmetic.
+
+                simplify.
+                linear_arithmetic.
+
+                exfalso. linear_arithmetic.
+            ---
+                pose proof (VarToNode st v0 v nvs H x n Heq).
+                pose proof (VarToNode st v0 v nvs H y n0 Heq0).
+                pose proof (symMulOf_correct st v0 v nvs n _ _ H H1 Heq1).
+                pose proof (symMulOf_correct st v0 v nvs n0 _ _ H H2 Heq2).
+                pose proof (VarToNodevals st v0 v nvs H x n Heq).
+                pose proof (VarToNodevals st v0 v nvs H y n0 Heq0).
+
+                rewrite H5 in H3.
+                rewrite H6 in H4.
+                invert H3.
+                invert H4.
+                rewrite H7, H8.
+
+                unfold product.
+
+                eapply merge_combine; eauto; simplify; linear_arithmetic.
+          -- exfalso; eauto.
+        ++ exfalso; eauto.
+
+      + cases (Vars st $? x); simplify.
+        ++ cases (Vars st $? y); simplify.
+          -- cases (NodesOut st $? n).
+            --- cases (NodesOut st $? n0).
+              +++ cases (n2).
+                  cases (n2 ==z 0).
+                  pose proof (VarToNode st v0 v nvs H x n Heq).
+                  pose proof (VarToNode st v0 v nvs H y n0 Heq0).
+                  pose proof (VarToNodevals st v0 v nvs H x n Heq).
+                  pose proof (VarToNodevals st v0 v nvs H y n0 Heq0).
+                  pose proof (OutVals st v0 v nvs H n n1 Heq1).
+                  pose proof (OutVals st v0 v nvs H n0 (SConst n2) Heq2).
+                  invert H5.
+                  invert H6.
+                  rewrite H3 in H8.
+                  invert H8.
+                  rewrite H7 in H4.
+                  invert H4.
+                  linear_arithmetic.
+
+                  pose proof (VarToNode st v0 v nvs H x n Heq).
+                  pose proof (VarToNode st v0 v nvs H y n0 Heq0).
+                  pose proof (VarToNodevals st v0 v nvs H x n Heq).
+                  pose proof (VarToNodevals st v0 v nvs H y n0 Heq0).
+                  pose proof (OutVals st v0 v nvs H n n1 Heq1).
+                  pose proof (OutVals st v0 v nvs H n0 (SConst n2) Heq2).
+                  invert H5.
+                  invert H6.
+                  rewrite H3 in H8.
+                  invert H8.
+                  rewrite H7 in H4.
+                  invert H4.
+                  simplify.
+                  rewrite H3.
+                  rewrite H7.
+                  linear_arithmetic.
+
+                  pose proof (VarToNode st v0 v nvs H x n Heq).
+                  pose proof (VarToNode st v0 v nvs H y n0 Heq0).
+                  pose proof (VarToNodevals st v0 v nvs H x n Heq).
+                  pose proof (VarToNodevals st v0 v nvs H y n0 Heq0).
+                  pose proof (OutVals st v0 v nvs H n n1 Heq1).
+                  pose proof (OutVals st v0 v nvs H n0 (SVar x0) Heq2).
+                  invert H5.
+                  invert H6.
+                  rewrite H3 in H8.
+                  invert H8.
+                  rewrite H7 in H4.
+                  invert H4.
+                  simplify.
+                  rewrite H3.
+                  rewrite H7.
+                  linear_arithmetic.
+
+                  pose proof (VarToNode st v0 v nvs H x n Heq).
+                  pose proof (VarToNode st v0 v nvs H y n0 Heq0).
+                  pose proof (VarToNodevals st v0 v nvs H x n Heq).
+                  pose proof (VarToNodevals st v0 v nvs H y n0 Heq0).
+                  pose proof (OutVals st v0 v nvs H n n1 Heq1).
+                  pose proof (OutVals st v0 v nvs H n0 (SAdd n2 args) Heq2).
+                  invert H5.
+                  invert H6.
+                  rewrite H3 in H8.
+                  invert H8.
+                  rewrite H7 in H4.
+                  invert H4.
+                  simplify.
+                  rewrite H3.
+                  rewrite H7.
+                  linear_arithmetic.
+
+                  pose proof (VarToNode st v0 v nvs H x n Heq).
+                  pose proof (VarToNode st v0 v nvs H y n0 Heq0).
+                  pose proof (VarToNodevals st v0 v nvs H x n Heq).
+                  pose proof (VarToNodevals st v0 v nvs H y n0 Heq0).
+                  pose proof (OutVals st v0 v nvs H n n1 Heq1).
+                  pose proof (OutVals st v0 v nvs H n0 (SMul n2 args) Heq2).
+                  invert H5.
+                  invert H6.
+                  rewrite H3 in H8.
+                  invert H8.
+                  rewrite H7 in H4.
+                  invert H4.
+                  simplify.
+                  rewrite H3.
+                  rewrite H7.
+                  linear_arithmetic.
+
+
+                  pose proof (VarToNode st v0 v nvs H x n Heq).
+                  pose proof (VarToNode st v0 v nvs H y n0 Heq0).
+                  pose proof (VarToNodevals st v0 v nvs H x n Heq).
+                  pose proof (VarToNodevals st v0 v nvs H y n0 Heq0).
+                  pose proof (OutVals st v0 v nvs H n n1 Heq1).
+                  pose proof (OutVals st v0 v nvs H n0 (SSub x0 y0) Heq2).
+                  invert H5.
+                  invert H6.
+                  rewrite H3 in H8.
+                  invert H8.
+                  rewrite H7 in H4.
+                  invert H4.
+                  simplify.
+                  rewrite H3.
+                  rewrite H7.
+                  linear_arithmetic.
+              +++
+                  pose proof (VarToNode st v0 v nvs H x n Heq).
+                  pose proof (VarToNode st v0 v nvs H y n0 Heq0).
+                  pose proof (VarToNodevals st v0 v nvs H x n Heq).
+                  pose proof (VarToNodevals st v0 v nvs H y n0 Heq0).
+
+                  exfalso. eauto.
+            ---
+                pose proof (VarToNode st v0 v nvs H x n Heq).
+                pose proof (VarToNode st v0 v nvs H y n0 Heq0).
+                pose proof (VarToNodevals st v0 v nvs H x n Heq).
+                pose proof (VarToNodevals st v0 v nvs H y n0 Heq0).
+
+                exfalso. eauto.
+          --  pose proof (VarToNode st v0 v nvs H x n Heq).
+              pose proof (VarToNodevals st v0 v nvs H x n Heq).
+
+              eapply varIsFine in H0; eauto.
+              exfalso. eauto.
+
+              exfalso. eauto.
+        ++  eapply varIsFine in H0; eauto.
+            exfalso. eauto.
+
+            exfalso. eauto.
+  Qed.
+
+  (* From this point out, things are getting more complicated, and we're not
+   * going to narrate the details (and all the proofs are already included). *)
+
+  Local Hint Resolve InToOut OutVals : core.
+
+  Definition node_kind_eq_dec : forall nk1 nk2 : node_kind, sumbool (nk1 = nk2) (nk1 <> nk2).
+  Proof.
+    decide equality.
+    apply Z.eq_dec.
+    apply var_eq.
+    apply list_eq_dec; apply Z.eq_dec.
+    apply Z.eq_dec.
+    apply list_eq_dec; apply Z.eq_dec.
+    apply Z.eq_dec.
+    apply Z.eq_dec.
+    apply Z.eq_dec.
+  Qed.
+
+  Lemma nodeKindInBounds_mono : forall n n' nk,
+      nodeKindInBounds n nk
+      -> n <= n'
+      -> nodeKindInBounds n' nk.
+  Proof.
+    simplify; cases nk; simplify; propositional; try linear_arithmetic.
+    eapply Forall_impl; eauto; simplify; linear_arithmetic.
+    eapply Forall_impl; eauto; simplify; linear_arithmetic.
+  Qed.
+
+  Lemma map_bound : forall bound (nvs1 nvs2 : nodeVals) args,
+      Forall (fun arg => arg < bound) args
+      -> (forall k, k < bound -> nvs1 $? k = nvs2 $? k)
+      -> map (fun nd => nvs1 $! nd) args = map (fun nd => nvs2 $! nd) args.
+  Proof.
+    induct args; simplify; auto.
+
+    invert H.
+    f_equal; auto.
+    rewrite H0 by assumption.
+    reflexivity.
+  Qed.
+
+  Lemma evalNodeKind_relevant : forall bound nk nvs1 nvs2 v,
+      nodeKindInBounds bound nk
+      -> (forall k, k < bound -> nvs1 $? k = nvs2 $? k)
+      -> evalNodeKind nvs1 v nk = evalNodeKind nvs2 v nk.
+  Proof.
+    simplify.
+    cases nk; simplify; propositional; auto.
+
+    f_equal.
+    eapply map_bound; eauto.
+
+    f_equal.
+    eapply map_bound; eauto.
+
+    rewrite !H0 by assumption.
+    reflexivity.
+  Qed.
+
+  Local Hint Resolve InBounds2 OutToIn includes_refl : core.
+
+  Lemma includes_add : forall A B (m : fmap A B) k v,
+      m $? k = None
+      -> m $<= m $+ (k, v).
+  Proof.
+    simplify.
+    apply includes_intro.
+    simplify.
+    assumption.
+  Qed.
+
+  Local Hint Resolve includes_add : core.
+
+  Definition node_kind_in_correct : forall st v0 v nvs nk,
+      compat st v0 v nvs
+      -> nodeKindInBounds st.(NextNode) nk
+      -> exists nvs', nvs $<= nvs'
+                      /\ compat (fst (node_kind_in st nk)) v0 v nvs'
+                      /\ (fst (node_kind_in st nk)).(NodesOut) $? snd (node_kind_in st nk) <> None
+                      /\ nvs' $? snd (node_kind_in st nk) = Some (evalNodeKind nvs' v0 nk).
+  Proof.
+    unfold node_kind_in; simplify.
+    cases (NodesIn st $? nk); simplify.
+
+    exists nvs; propositional; eauto.
+    eapply InToOut in Heq; eauto.
+    equality.
+
+    exists (nvs $+ (st.(NextNode), evalNodeKind nvs v0 nk)).
+    simplify; propositional; try equality.
+
+    apply includes_add.
+    cases (nvs $? NextNode st); auto.
+    assert (nvs $? NextNode st <> None) by equality.
+    eapply OutValsInv in H1; eauto.
+    cases (NodesOut st $? NextNode st); try equality.
+    eapply InBounds1 in Heq1; eauto.
+    linear_arithmetic.
+
+    constructor; simplify; eauto using InBounds1.
+
+    cases (node_kind_eq_dec nk nk0); subst; simplify.
+    cases (Z.eq_dec (NextNode st) nd); subst; simplify; auto.
+    eapply OutToIn in H1; eauto; equality.
+    cases (Z.eq_dec (NextNode st) nd); subst; simplify; auto.
+    equality.
+    eauto using OutToIn.
+
+    cases (Z.eq_dec (NextNode st) nd); subst; simplify.
+    cases (node_kind_eq_dec nk nk0); subst; simplify; auto.
+    eapply InToOut in H1; eauto.
+    eapply InBounds1 in H1; eauto.
+    linear_arithmetic.
+    cases (node_kind_eq_dec nk nk0); subst; simplify; auto.
+    equality.
+    eauto.
+
+    cases (Z.eq_dec (NextNode st) nd); subst; simplify.
+    linear_arithmetic.
+    eapply InBounds1 in H1; eauto.
+    linear_arithmetic.
+
+    cases (node_kind_eq_dec nk nk0); subst; simplify.
+    eapply nodeKindInBounds_mono; eauto.
+    linear_arithmetic.
+    eapply InBounds2 in H1; eauto.
+    eapply nodeKindInBounds_mono; eauto.
+    linear_arithmetic.
+
+    cases (Z.eq_dec (NextNode st) nd); subst; simplify.
+    invert H1.
+    f_equal.
+    eapply evalNodeKind_relevant; eauto.
+    simplify.
+    assert (k <> NextNode st) by linear_arithmetic.
+    simplify.
+    reflexivity.
+    erewrite OutVals; eauto.
+    f_equal.
+    eapply evalNodeKind_relevant; eauto.
+    simplify.
+    cases (Z.eq_dec (NextNode st) k); subst; simplify; auto.
+    linear_arithmetic.
+
+    cases (Z.eq_dec (NextNode st) nd); subst; simplify; eauto; try equality.
+    eapply OutValsInv in H1; eauto.
+
+    cases (Z.eq_dec (NextNode st) nd); subst; simplify; eauto.
+    eapply VarToNode in H1; eauto.
+    cases (NodesOut st $? NextNode st); equality.
+
+    assert (nd <> NextNode st).
+    eapply VarToNode in H1; eauto.
+    cases (NodesOut st $? NextNode st); simplify; try equality.
+    eapply InBounds1 in Heq0; eauto.
+    linear_arithmetic.
+    simplify.
+    eauto using VarToNodevals.
+
+    f_equal.
+    eapply evalNodeKind_relevant; eauto.
+    simplify.
+    assert (k <> NextNode st) by linear_arithmetic.
+    simplify.
+    reflexivity.
+  Qed.
+
+  Lemma VarInBounds : forall st v0 v nvs x n,
+      compat st v0 v nvs
+      -> Vars st $? x = Some n
+      -> n < NextNode st.
+  Proof.
+    simplify.
+    eapply VarToNode in H0; eauto.
+    cases (NodesOut st $? n); try equality.
+    eapply InBounds1; eauto.
+  Qed.
+
+  Local Hint Resolve VarInBounds : core.
+
+  Lemma symAddOf_bounds : forall st v0 v nvs n z l,
+      compat st v0 v nvs
+      -> symAddOf st n = (z, l)
+      -> st.(NodesOut) $? n <> None
+      -> Forall (fun arg => arg < st.(NextNode)) l.
+  Proof.
+    unfold symAddOf; simplify.
+    repeat match goal with
+           | [ H : (_, _) = (_, _) |- _ ] => invert H
+           | [ H : match ?E with _ => _ end = _ |- _ ] => cases E
+           | [ H : _.(NodesOut) $? _ = Some _ |- _ ] => solve [ eapply InBounds1 in H; eauto ]
+           end; auto; try equality.
+    eapply OutToIn in Heq; eauto.
+    eapply InBounds2 in Heq; eauto.
+  Qed.
+
+  Lemma symMulOf_bounds : forall st v0 v nvs n z l,
+      compat st v0 v nvs
+      -> symMulOf st n = (z, l)
+      -> st.(NodesOut) $? n <> None
+      -> Forall (fun arg => arg < st.(NextNode)) l.
+  Proof.
+    unfold symMulOf; simplify.
+    repeat match goal with
+           | [ H : (_, _) = (_, _) |- _ ] => invert H
+           | [ H : match ?E with _ => _ end = _ |- _ ] => cases E
+           | [ H : _.(NodesOut) $? _ = Some _ |- _ ] => solve [ eapply InBounds1 in H; eauto ]
+           end; auto; try equality.
+    eapply OutToIn in Heq; eauto.
+    eapply InBounds2 in Heq; eauto.
+  Qed.
+
+  Lemma merge_property : forall P l1 l2,
+      Forall P l1
+      -> Forall P l2
+      -> Forall P (ZSort.merge l1 l2).
+  Proof.
+    induct l1; induct l2; simplify; auto.
+    invert H.
+    invert H0.
+    cases (a <=? a0); auto.
+  Qed.
+
+  Local Hint Resolve merge_property symAddOf_bounds symMulOf_bounds : core.
+
+  Lemma in_bounds_rhs : forall st v0 v nvs r,
+      compat st v0 v nvs
+      -> rhsReads r \subseteq dom st.(Vars)
+      -> nodeKindInBounds st.(NextNode) (kindOfRhs st r).
+  Proof.
+    simplify; cases r; simplify; auto.
+    repeat match goal with
+           | [ |- nodeKindInBounds _ (match ?E with _ => _ end) ] => cases E
+           end; simplify; propositional; eauto 6.
+  Qed.
+
+  Local Hint Resolve in_bounds_rhs : core.
+
+  Lemma node_kind_in_Vars : forall st nk st' nd,
+      node_kind_in st nk = (st', nd)
+      -> Vars st' = Vars st.
+  Proof.
+    unfold node_kind_in; simplify.
+    cases (NodesIn st $? nk); try equality.
+    invert H.
+    reflexivity.
+  Qed.
+
+  Lemma node_kind_in_NodesOut : forall st nk st' nd v0 v nvs,
+      compat st v0 v nvs
+      -> node_kind_in st nk = (st', nd)
+      -> st.(NodesOut) $<= st'.(NodesOut).
+  Proof.
+    unfold node_kind_in; simplify.
+    cases (NodesIn st $? nk); try equality.
+    invert H0.
+    auto.
+    invert H0.
+    simplify.
+    apply includes_add.
+    cases (NodesOut st $? NextNode st); auto.
+    eapply InBounds1 in Heq0; eauto.
+    linear_arithmetic.
+  Qed.
+
+  Local Hint Resolve node_kind_in_Vars node_kind_in_NodesOut : core.
+
+  Lemma symAddOf_mono : forall st v0 v nvs nd st' x,
+      compat st v0 v nvs
+      -> st.(NodesOut) $<= st'.(NodesOut)
+      -> st.(Vars) = st'.(Vars)
+      -> st.(Vars) $? x = Some nd
+      -> symAddOf st' nd = symAddOf st nd.
+  Proof.
+    unfold symAddOf; simplify.
+    cases (NodesOut st $? nd).
+    erewrite includes_lookup; eauto.
+    eapply VarToNode in H2; eauto.
+    equality.
+  Qed.
+
+  Lemma symMulOf_mono : forall st v0 v nvs nd st' x,
+      compat st v0 v nvs
+      -> st.(NodesOut) $<= st'.(NodesOut)
+      -> st.(Vars) = st'.(Vars)
+      -> st.(Vars) $? x = Some nd
+      -> symMulOf st' nd = symMulOf st nd.
+  Proof.
+    unfold symMulOf; simplify.
+    cases (NodesOut st $? nd).
+    erewrite includes_lookup; eauto.
+    eapply VarToNode in H2; eauto.
+    equality.
+  Qed.
+
+  Lemma kindOfRhs_mono : forall st v0 v nvs r st',
+      compat st v0 v nvs
+      -> rhsReads r \subseteq dom (Vars st)
+      -> st.(NodesOut) $<= st'.(NodesOut)
+      -> st.(Vars) = st'.(Vars)
+      -> kindOfRhs st' r = kindOfRhs st r.
+  Proof.
+    simplify; case r; simplify; auto.
+    rewrite <- H2.
+    repeat match goal with
+           | [ |- _ = match ?E with _ => _ end ] => cases E
+           end; auto.
+
+    erewrite symAddOf_mono by eauto.
+    rewrite Heq1.
+    erewrite symAddOf_mono by eauto.
+    rewrite Heq2.
+    rewrite Heq3.
+    reflexivity.
+
+    erewrite symAddOf_mono by eauto.
+    rewrite Heq1.
+    erewrite symAddOf_mono by eauto.
+    rewrite Heq2.
+    rewrite Heq3.
+    reflexivity.
+
+    erewrite symMulOf_mono by eauto.
+    rewrite Heq1.
+    erewrite symMulOf_mono by eauto.
+    rewrite Heq2.
+    rewrite Heq3.
+    reflexivity.
+
+    erewrite symMulOf_mono by eauto.
+    rewrite Heq1.
+    erewrite symMulOf_mono by eauto.
+    rewrite Heq2.
+    rewrite Heq3.
+    reflexivity.
+
+    repeat erewrite includes_lookup by eauto.
+    simplify.
+    cases (n2 ==z 0); equality.
+
+    repeat erewrite includes_lookup by eauto.
+    simplify.
+    cases (n2 ==z 0); equality.
+
+    repeat erewrite includes_lookup by eauto.
+    simplify.
+    reflexivity.
+
+    repeat erewrite includes_lookup by eauto.
+    simplify.
+    reflexivity.
+
+    repeat erewrite includes_lookup by eauto.
+    simplify.
+    reflexivity.
+
+    repeat erewrite includes_lookup by eauto.
+    simplify.
+    reflexivity.
+
+    eapply VarToNode in Heq0; eauto.
+    equality.
+
+    eapply VarToNode in Heq; eauto.
+    equality.
+  Qed.
+
+  Lemma symInstr_correct : forall i st v0 v nvs,
+      compat st v0 v nvs
+      -> rhsReads (Rhs i) \subseteq dom st.(Vars)
+      -> exists nvs', nvs $<= nvs' /\ compat (symInstr st i) v0 (evalInstr v i) nvs'.
+  Proof.
+    unfold symInstr, evalInstr; simplify.
+    cases (node_kind_in st (kindOfRhs st (Rhs i))).
+    specialize (node_kind_in_correct _ _ _ _ (kindOfRhs st (Rhs i)) H).
+    rewrite Heq; simplify.
+    assert (nodeKindInBounds (NextNode st) (kindOfRhs st (Rhs i))) by eauto.
+    propositional.
+    invert H3; propositional.
+    exists x; propositional.
+    constructor; simplify; eauto using InBounds1, OutValsInv.
+    cases (x0 ==v Lhs i); subst; simplify; eauto.
+    equality.
+    cases (x0 ==v Lhs i); subst; simplify; eauto using VarToNodevals.
+    invert H5.
+    rewrite H6.
+    f_equal.
+    replace (kindOfRhs st (Rhs i)) with (kindOfRhs s (Rhs i)).
+    apply kindOfRhs_correct; auto.
+    erewrite node_kind_in_Vars by eauto.
+    assumption.
+    eapply kindOfRhs_mono; eauto.
+    symmetry; eauto.
+  Qed.
+
+  Theorem includes_trans : forall A B (m1 m2 m3 : fmap A B),
+      m1 $<= m2
+      -> m2 $<= m3
+      -> m1 $<= m3.
+  Proof.
+    simplify; apply includes_intro; eauto.
+  Qed.
+
+  Lemma symProg_correct : forall pr st v0 v nvs,
+      compat st v0 v nvs
+      -> progReads pr \subseteq dom (Vars st)
+      -> exists nvs', nvs $<= nvs' /\ compat (symProg pr st) v0 (evalProg pr v) nvs'.
+  Proof.
+    induct pr; simplify; propositional; eauto.
+
+    apply symInstr_correct with (i := a) in H.
+    2: cases a; sets.
+    invert H; propositional.
+    eapply IHpr in H2.
+    invert H2; propositional.
+    exists x0; propositional; eauto using includes_trans.
+    cases (node_kind_in st (kindOfRhs st (Rhs a))); simplify.
+    assert (s.(Vars) = st.(Vars)).
+    unfold node_kind_in in Heq.
+    cases (st.(NodesIn) $? kindOfRhs st (Rhs a)); simplify.
+    equality.
+    invert Heq.
+    reflexivity.
+    unfold symInstr.
+    rewrite Heq.
+    simplify.
+    cases a; simplify.
+    sets.
+    cases (Lhs0 ==v x0); auto.
+    right.
+    rewrite H1.
+    apply H0; propositional.
+  Qed.
+
+  Definition initNodevals (v : valuation) : nodeVals :=
+    $0 $+ (0, v $! "a") $+ (1, v $! "b") $+ (2, v $! "c").
+
+  Lemma compat_initVars : forall v,
+      compat initial v v (initNodevals v).
+  Proof.
+    unfold initNodevals; constructor; simplify;
+      repeat match goal with
+             | [ H: Some _ = Some _ |- _ ] => invert H
+             | [ |- context[(_ $+ (?x, _)) $? ?y] ] => cases (node_kind_eq_dec x y); subst; simplify
+             | [ |- context[(_ $+ (?x, _)) $? ?y] ] => cases (Z.eq_dec x y); subst; simplify
+             | [ _ : context[(_ $+ (?x, _)) $? ?y] |- _ ] => cases (Z.eq_dec x y); subst; simplify
+             | [ _ : context[(_ $+ (?x, _)) $? ?y] |- _ ] => cases (node_kind_eq_dec x y); subst; simplify
+             | [ _ : context[(_ $+ (?x, _)) $? ?y] |- _ ] => cases (string_dec x y); subst; simplify
+             end; equality || linear_arithmetic.
+  Qed.
+
+  Lemma compat_redoVars : forall st v v' nvs,
+      initNodevals v $<= nvs
+      -> compat st v v' nvs
+      -> compat (redoVars st) v v nvs.
+  Proof.
+    simplify.
+    constructor; simplify; eauto using InBounds1, OutValsInv.
+    repeat match goal with
+           | [ H: Some _ = Some _ |- _ ] => invert H
+           | [ _ : context[(_ $+ (?x, _)) $? ?y] |- _ ] => cases (string_dec x y); subst; simplify
+           end;
+      unfold initNodevals in *;
+      eapply OutValsInv; eauto;
+      erewrite includes_lookup; try apply H; simplify; eauto; equality.
+    repeat match goal with
+           | [ H: Some _ = Some _ |- _ ] => invert H
+           | [ _ : context[(_ $+ (?x, _)) $? ?y] |- _ ] => cases (string_dec x y); subst; simplify
+           end;
+    unfold initNodevals in *;
+      erewrite includes_lookup; try apply H; simplify; eauto; equality.
+  Qed.
+
+  Local Hint Resolve compat_initVars compat_redoVars : core.
 
   Theorem equivalent_correct : forall pr1 pr2,
       equivalent pr1 pr2 = true
       -> (progReads pr1 \cup progReads pr2) \subseteq inputs
       -> forall v, evalProg pr1 v $! "out" = evalProg pr2 v $! "out".
   Proof.
-  Admitted.
+    intros.
+    unfold equivalent in H.
+    repeat match goal with
+           | [ H : match ?E with _ => _ end = _ |- _ ] => cases E; try equality
+           end.
+    assert (exists nvs, initNodevals v $<= nvs /\ compat (symProg pr1 initial) v (evalProg pr1 v) nvs).
+    apply symProg_correct; simplify; auto.
+    unfold inputs in *; sets; first_order.
+    invert H1; propositional.
+    assert (exists nvs', x $<= nvs' /\ compat (symProg pr2 (redoVars (symProg pr1 initial))) v (evalProg pr2 v) nvs').
+    apply symProg_correct; simplify; eauto.
+    generalize H0; clear; sets; first_order.
+    invert H2; propositional.
+    eapply VarToNodevals in Heq; eauto.
+    eapply VarToNodevals in Heq0; eauto.
+    apply Z.eqb_eq in H; subst.
+    erewrite includes_lookup in Heq0; try apply H2; eauto.
+    equality.
+  Qed.
+
 End Impl.
 
 Module ImplCorrect : Pset10Sig.S := Impl.
